Define integer maximum in integerScript, and also replace all internal uses of INT_ADD_SYM with INT_ADD_COMM.  In Cooper.sig allow for export of useful non_presburger_subterms.

src/integer/Cooper.sig
@@ -1,13 +1,14 @@
-signature Cooper = 
+signature Cooper =
 sig
   type term = Term.term
   type thm = Thm.thm
   type conv = Abbrev.conv
   type tactic = Abbrev.tactic
 
-  val COOPER_CONV   : conv
-  val COOPER_PROVE  : conv 
-  val COOPER_TAC    : tactic
-  val is_presburger : term -> bool
+  val COOPER_CONV                 : conv
+  val COOPER_PROVE                : conv
+  val COOPER_TAC                  : tactic
+  val is_presburger               : term -> bool
+  val non_presburger_subterms     : term -> term list
   val decide_pure_presburger_term : term -> thm
 end
